

Problem 1:

$$\begin{cases} x - 3y + 2z = -1 \\ 2x - 5y + 9z = 10 \\ 2x - 5y + 6z = 4 \end{cases} \quad (1)$$

(a) Is $(x, y, z) = (35, 12, 0)$ a solution of (1)?

We can either check directly on (1) or put it first in RREF form since this is asked later.

We will check this directly:

In the third equation:

$$2 \cdot 35 - 5 \cdot 12 + 6 \cdot 0 \neq 4$$

so $(35, 12, 0)$ is not a solution of (1).

(b) Give the expression of the augmented matrix corresponding to (1)

$$\left[\begin{array}{ccc|c} 1 & -3 & 2 & -1 \\ 2 & -5 & 9 & 10 \\ 2 & -5 & 6 & 4 \end{array} \right]$$

(C)

$$\left[\begin{array}{ccc|c} 1 & -3 & 2 & -1 \\ 2 & -5 & 9 & 10 \\ 2 & -5 & 6 & 4 \end{array} \right] \xrightarrow{\substack{R_2 - 2R_1 \\ R_3 - 2R_1}} \left[\begin{array}{ccc|c} 1 & -3 & 2 & -1 \\ 0 & 1 & 5 & 12 \\ 0 & 1 & 2 & 6 \end{array} \right]$$

$$\xrightarrow{\substack{R_1 + 3R_2 \\ R_3 - R_2}} \left[\begin{array}{ccc|c} 1 & 0 & 17 & 35 \\ 0 & 1 & 5 & 12 \\ 0 & 0 & -3 & -6 \end{array} \right] \xrightarrow{R_3 / -3} \left[\begin{array}{ccc|c} 1 & 0 & 17 & 35 \\ 0 & 1 & 5 & 12 \\ 0 & 0 & 1 & 2 \end{array} \right]$$

$$\xrightarrow{\substack{R_2 - 5R_3 \\ R_1 - 17R_3}} \left[\begin{array}{ccc|c} 1 & 0 & 0 & 1 \\ 0 & 1 & 0 & 2 \\ 0 & 0 & 1 & 2 \end{array} \right]$$

$\Rightarrow \quad x = 1 \quad \Rightarrow \quad (1, 2, 2) \text{ is the unique solution.}$
 $y = 2$
 $z = 2$

Problem 2: $A = \begin{bmatrix} 1 & 2 & 5 \\ 4 & 3 & 5 \end{bmatrix}$

(a) Determine the range of A .

The range is the column space $\text{span} \left\{ \begin{bmatrix} 1 \\ 4 \end{bmatrix}, \begin{bmatrix} 2 \\ 3 \end{bmatrix}, \begin{bmatrix} 5 \\ 5 \end{bmatrix} \right\}$

We need to check linear independence (which we can already see since we have 3 vectors in \mathbb{R}^2).

We will put A in RREF

$$A = \begin{bmatrix} 1 & 2 & 5 \\ 4 & 3 & 5 \end{bmatrix} \xrightarrow{R_2 - 4R_1} \begin{bmatrix} 1 & 2 & 5 \\ 0 & -5 & -15 \end{bmatrix} \xrightarrow{R_2 / -5} \begin{bmatrix} 1 & 2 & 5 \\ 0 & 1 & 3 \end{bmatrix}$$

$$\xrightarrow{R_1 - 2R_2} \begin{bmatrix} 1 & 0 & -1 \\ 0 & 1 & 3 \end{bmatrix}$$

linear independent columns so we need the corresponding columns of the original matrix

$$\Rightarrow \text{range}(A) = \text{span} \left\{ \begin{bmatrix} 1 \\ 4 \end{bmatrix}, \begin{bmatrix} 2 \\ 3 \end{bmatrix} \right\} = \mathbb{R}^2$$

(B) Recall that the rank is the maximal number of non-zero linear independent rows or columns.

Since we only have two rows. $\text{rank}(A) \leq 2$.

By putting the matrix in RREF we already proved that it has exactly two non-zero linearly independent columns. This means that $\text{rank}(A) = 2$.

(C) Give a basis for $\text{null}(A)$

We solve $A\bar{x} = 0$ for $\bar{x} = \begin{pmatrix} x \\ y \\ z \end{pmatrix}$

$$\Rightarrow \begin{bmatrix} 1 & 2 & 5 \\ 4 & 3 & 5 \end{bmatrix} \begin{bmatrix} x \\ y \\ z \end{bmatrix} = \begin{bmatrix} 0 \\ 0 \end{bmatrix}$$

$$\Rightarrow \begin{aligned} x + 2y + 5z &= 0 \\ 4x + 3y + 5z &= 0 \end{aligned} \quad \left(\text{solve for any variable!} \right)$$

$$\Rightarrow \begin{aligned} y &= -3x \\ z &= x \end{aligned}$$

$$\Rightarrow x + 2y = 4x + 3y$$

$$\Rightarrow 3x + y = 0 \Rightarrow y = -3x$$

$$\text{null}(A) = \text{span} \left(\left\{ \begin{bmatrix} x \\ y \\ z \end{bmatrix} \in \mathbb{R}^3 : \begin{aligned} x + 2y + 5z &= 0 \\ 4x + 3y + 5z &= 0 \end{aligned} \right\} \right)$$

$$= \text{span} \left(\left\{ \begin{bmatrix} x \\ y \\ z \end{bmatrix} \in \mathbb{R}^3 : \begin{aligned} y &= -3x \\ y &= z \end{aligned} \right\} \right)$$

$$= \text{span} \left(\left\{ \begin{bmatrix} x \\ -3x \\ x \end{bmatrix} \in \mathbb{R}^3 \right\} \right)$$

$$= \text{span} \left(\left\{ x \begin{bmatrix} 1 \\ -3 \\ 1 \end{bmatrix} \in \mathbb{R}^3 \right\} \right)$$

$$\text{has a basis } \left\{ \begin{bmatrix} 1 \\ -3 \\ 1 \end{bmatrix} \right\}$$

(d) Determine $\text{nullity}(A)$.

$$\text{nullity}(A) = \dim \text{null}(A) = 1 \quad \text{as seen above.}$$

Problem 3:

$$\begin{aligned} \text{(a)} \quad \det(A^{-1} B A) &= \det(A^{-1}) \cdot \det(B) \cdot \det(A) \\ &= \frac{1}{\det(A)} \cdot \det(B) \cdot \det(A) \\ &= \det(B) \end{aligned}$$

$$= \det(B)$$

$$= -3$$

$$\begin{aligned} \text{(b)} \quad \det(A' B A) &= \det(A') \cdot \det(B) \cdot \det(A) \\ &= \det(A) \cdot \det(B) \cdot \det(A) \\ &= 4 \cdot (-3) \cdot 4 \\ &= -48 \end{aligned}$$

$$(c) \det(B^5) = \det(B)^5 = (-3)^5$$

Problem 4:

• For $b=d=0$ it contains the zero vector $\begin{bmatrix} 0 \\ 0 \\ 0 \\ 0 \end{bmatrix}$

• Let $\begin{bmatrix} b_1 - 5d_1 \\ 2b_1 \\ 2d_1 \\ d_1 \end{bmatrix}, \begin{bmatrix} b_2 - 5d_2 \\ 2b_2 \\ 2d_2 \\ d_2 \end{bmatrix} \in S$

then

$$\begin{bmatrix} b_1 - 5d_1 \\ 2b_1 \\ 2d_1 \\ d_1 \end{bmatrix} + \begin{bmatrix} b_2 - 5d_2 \\ 2b_2 \\ 2d_2 \\ d_2 \end{bmatrix} = \begin{bmatrix} (b_1 + b_2) - 5(d_1 + d_2) \\ 2(b_1 + b_2) \\ 2(d_1 + d_2) \\ (d_1 + d_2) \end{bmatrix} \in S$$

• Let $c \in \mathbb{R}$ and $\begin{bmatrix} b - 5d \\ 2b \\ 2d \\ d \end{bmatrix} \in S$.

$$\text{Then } c \cdot \begin{bmatrix} b & -sd \\ 2b \\ 2d \\ d \end{bmatrix} = \begin{bmatrix} (cb) - s(cd) \\ 2(cb) \\ 2(cd) \\ (cd) \end{bmatrix} \in S$$

$\Rightarrow S$ is a subspace of \mathbb{R}^4

Problem 5:

I first put A in RREF

$$A \text{ has RREF } \begin{bmatrix} 1 & 0 & 1 \\ 0 & 1 & 1/2 \\ 0 & 0 & 0 \end{bmatrix}$$

so a basis for the range are the first two columns of the original A which is $\left\{ \begin{bmatrix} -8 \\ 6 \\ 4 \end{bmatrix}, \begin{bmatrix} -2 \\ 4 \\ 0 \end{bmatrix} \right\}$

Then let $d_1, d_2 \in \mathbb{R}$:

$$d_1 \begin{bmatrix} -8 \\ 6 \\ 4 \end{bmatrix} + d_2 \begin{bmatrix} -2 \\ 4 \\ 0 \end{bmatrix} = b = \begin{bmatrix} 2 \\ 1 \\ -2 \end{bmatrix}$$

$$\Rightarrow \begin{bmatrix} -8d_1 - 2d_2 \\ 6d_1 + 4d_2 \\ 4d_1 \end{bmatrix} = \begin{bmatrix} 2 \\ 1 \\ -2 \end{bmatrix}$$

$$\Rightarrow d_1 = -\frac{1}{2}, d_2 = 1$$

So b is in the range of A .

Problem 6:

$$\begin{aligned} (\alpha) \det(A - \lambda I) &= \det \begin{bmatrix} 2 - \lambda & 4 \\ 1 & 2 - \lambda \end{bmatrix} \\ &= (2 - \lambda)^2 - 4 \\ &= 4 - 4\lambda + \lambda^2 - 4 \\ &= \lambda^2 - 4\lambda \\ &= \lambda(\lambda - 4) \end{aligned}$$

$$\Rightarrow \det(A - \lambda I) = 0 \Rightarrow \lambda = 0 \quad (\text{simple roots}) \\ \text{or } \lambda = 4$$

$\Rightarrow \lambda = 0$ is an eigenvalue with algebraic multiplicity 1
 $\lambda = 4$ is an eigenvalue with algebraic multiplicity 1

(B) For $\lambda = 0$:

$$(A - \lambda I_2) \begin{bmatrix} x \\ y \end{bmatrix} = \begin{bmatrix} 0 \\ 0 \end{bmatrix}$$

$$A \begin{bmatrix} x \\ y \end{bmatrix} = \begin{bmatrix} 0 \\ 0 \end{bmatrix} \quad (\text{null}(A))$$

$$\begin{bmatrix} 2 & 4 \\ 1 & 2 \end{bmatrix} \begin{bmatrix} x \\ y \end{bmatrix} = \begin{bmatrix} 0 \\ 0 \end{bmatrix}$$

$$\begin{aligned} 2x + 4y &= 0 & \Leftrightarrow & x = -2y \\ x + 2y &= 0 \end{aligned}$$

$$E_0 = \text{span} \left(\left\{ \begin{bmatrix} x \\ y \end{bmatrix} \in \mathbb{R}^2 : x = -2y \right\} \right)$$

$$= \text{span} \left(\left\{ \begin{bmatrix} -2y \\ y \end{bmatrix} \in \mathbb{R}^2 \right\} \right)$$

$$= \text{span} \left(\left\{ y \begin{bmatrix} -2 \\ 1 \end{bmatrix} \in \mathbb{R}^2 \right\} \right)$$

$$= \text{span} \left(\left\{ \begin{bmatrix} -2 \\ 1 \end{bmatrix} \right\} \right) \Rightarrow \left\{ \begin{bmatrix} -2 \\ 1 \end{bmatrix} \right\} \text{ is a basis}$$

and $\lambda = 0$ has geometric multiplicity 1 as the dimension of the eigenspace is 1.

For $\lambda = 4$

$$(A - 4I_2) \begin{bmatrix} x \\ y \end{bmatrix} = \begin{bmatrix} 0 \\ 0 \end{bmatrix}$$

$$\begin{bmatrix} -2 & 4 \\ 1 & -2 \end{bmatrix} \begin{bmatrix} x \\ y \end{bmatrix} = \begin{bmatrix} 0 \\ 0 \end{bmatrix}$$

$$\Rightarrow \begin{bmatrix} -2x + 4y \\ x - 2y \end{bmatrix} = \begin{bmatrix} 0 \\ 0 \end{bmatrix}$$

$$\Rightarrow \begin{array}{l} -2x + 4y = 0 \\ x - 2y = 0 \end{array} \quad (\Rightarrow) \quad x = 2y$$

$$E_4 = \text{span} \left(\left\{ \begin{bmatrix} x \\ y \end{bmatrix} \in \mathbb{R}^2 : x = 2y \right\} \right)$$

$$= \text{span} \left(\left\{ y \begin{bmatrix} 2 \\ 1 \end{bmatrix} \in \mathbb{R}^2 \right\} \right)$$

$$\Rightarrow \text{a basis is } \left\{ \begin{bmatrix} 2 \\ 1 \end{bmatrix} \right\} \text{ with geometric multiplicity 1.}$$

(c) For $0 \neq u \in E_0$ then $Au = 0 \cdot u = 0$
this is $\text{null}(A)$.

For $0 \neq u \in E_4$ then $Au = 4 \cdot u$

(d) We set $P := \begin{bmatrix} -2 & 2 \\ 1 & 1 \end{bmatrix}$ a matrix with

the eigenvectors. Then we know that

$$P^{-1} A P = D = \begin{bmatrix} 0 & 0 \\ 0 & 4 \end{bmatrix}$$

$$\Rightarrow A = P D P^{-1}$$

$$\text{Consider } D^{1/2} := \begin{bmatrix} 0 & 0 \\ 0 & \sqrt{4} \end{bmatrix} = \begin{bmatrix} 0 & 0 \\ 0 & 2 \end{bmatrix}$$

$$\text{Then } A^{1/2} = P D^{1/2} P^{-1}$$

$$\begin{aligned} A^{1/2} \cdot A^{1/2} &= P D^{1/2} P^{-1} \cdot P D^{1/2} P^{-1} = P D^{1/2} \cdot D^{1/2} P^{-1} \\ &= A. \end{aligned}$$

Problem 7:

(a) True: $(AB)^{-1} = B^{-1} \cdot A^{-1}$

(b) False: α basis is not unique, dimension is

(c) True: $\dim \mathbb{R}^n = n$

(d) False: $A = \begin{pmatrix} -1 & 0 \\ 0 & 2 \end{pmatrix}, B = \begin{pmatrix} 0 & 1 \\ 0 & 3 \end{pmatrix}$

(e) False: Counterexample: $A = \begin{pmatrix} 1 & 0 \\ 0 & 2 \end{pmatrix}$

with eigenvalues 1, 2 but $1+2=3$ is not an eigenvalue.

Extra exercise with 2-dimensional eigenspace:

$$A = \begin{bmatrix} 2 & 0 & -2 \\ 0 & 3 & 0 \\ 0 & 0 & 3 \end{bmatrix}$$

$$\det(A - \lambda I) = 0 \quad (\Rightarrow) \quad (\lambda - 3)^2 (\lambda - 2) = 0$$

$$\Rightarrow \lambda = 3 \quad \text{or} \quad \lambda = 2.$$

We will do the $n=3$ case because it has a 2-dimensional eigenspace.

$$(A - 3I_3) \begin{bmatrix} x \\ y \\ z \end{bmatrix} = \begin{bmatrix} 0 \\ 0 \\ 0 \end{bmatrix}$$

$$\begin{bmatrix} -1 & 0 & -2 \\ 0 & 0 & 0 \\ 0 & 0 & 0 \end{bmatrix} \begin{bmatrix} x \\ y \\ z \end{bmatrix} = \begin{bmatrix} 0 \\ 0 \\ 0 \end{bmatrix}$$

$$\Leftrightarrow -x - 2z = 0.$$

$$\Leftrightarrow x = -2z$$

$$E_3 = \text{span} \left(\left\{ \begin{bmatrix} x \\ y \\ z \end{bmatrix} \in \mathbb{R}^3 : x = -2z \right\} \right)$$

$$= \text{span} \left(\left\{ \begin{bmatrix} -2z \\ 0 \\ z \end{bmatrix} + \begin{bmatrix} 0 \\ y \\ 0 \end{bmatrix} \in \mathbb{R}^3 \right\} \right)$$

$$= \text{span} \left(\left\{ z \begin{bmatrix} -2 \\ 0 \\ 1 \end{bmatrix} + y \begin{bmatrix} 0 \\ 1 \\ 0 \end{bmatrix} \in \mathbb{R}^3 \right\} \right)$$

$$\Rightarrow \text{a basis is } \left\{ \begin{bmatrix} -2 \\ 0 \\ 1 \end{bmatrix}, \begin{bmatrix} 0 \\ 1 \\ 0 \end{bmatrix} \right\}$$